@prefix audit: <https://w3id.org/ai-audit#>.
@prefix : <https://w3id.org/ai-audit/question#> .
@prefix owl:   <http://www.w3.org/2002/07/owl#> .
@prefix rdf:   <http://www.w3.org/1999/02/22-rdf-syntax-ns#> .
@prefix rdfs:  <http://www.w3.org/2000/01/rdf-schema#> .
@prefix xsd:   <http://www.w3.org/2001/XMLSchema#> .
@prefix dcterms: <http://purl.org/dc/terms/> .
@prefix pplan: <http://purl.org/net/p-plan#> .
@base <https://w3id.org/ai-audit/question#> .

: a owl:Ontology ;
  dcterms:title "AuditOps – Questions Module"@en ;
  dcterms:description "Vocabulary for representing audit questions, their types, and mappings to workflow steps and trace templates. "@en ;
  dcterms:abstract "This ontology describes audit questions and their relationships to audit criteria, and evidence. 
  It supports the structured formulation and reuse of questions across different audit contexts."; @en
  dcterms:creator "Laura Waltersdorfer" ;
  dcterms:contributor "Gregor Käfer", "Fajar J. Ekaputra", "Marta Sabou", "Tomasz Miksa";
  dcterms:license <https://creativecommons.org/licenses/by/4.0/>;
  owl:versionInfo "1.0.0" .

### Audit questions #############################################################

###  https://w3id.org/ai-audit/question#AuditQuestion
<https://w3id.org/ai-audit/question#AuditQuestion> a owl:Class ;
  rdfs:label "Audit Question"@en ;
  rdfs:comment "A natural-language audit question represented as a node to enable mapping to steps and trace templates."@en .

###  https://w3id.org/ai-audit/question#AuditQuestionType
<https://w3id.org/ai-audit/question#AuditQuestionType> a owl:Class ;
  rdfs:label "Audit Question Type"@en ;
  rdfs:comment "Audit question categories (e.g., lineage, temporal, location, attribute/property, aggregation)."@en .

###  https://w3id.org/ai-audit/question#questionType
<https://w3id.org/ai-audit/question#questionType> a owl:ObjectProperty ;
  rdfs:label "question type"@en ;
  rdfs:comment "Assigns a question to a question type."@en ;
  rdfs:domain :AuditQuestion ;
  rdfs:range :AuditQuestionType .



###  https://w3id.org/ai-audit/question#appliesToStep
<https://w3id.org/ai-audit/question#appliesToStep> a owl:ObjectProperty ;
  rdfs:label "applies to step"@en ;
  rdfs:comment "Indicates which workflow steps can provide evidence for answering the question."@en ;
  rdfs:domain :AuditQuestion ;
  rdfs:range pplan:Step .

###  https://w3id.org/ai-audit/question#appliesToPlan
<https://w3id.org/ai-audit/question#appliesToPlan> a owl:ObjectProperty ;
  rdfs:label "applies to plan"@en ;
  rdfs:comment "Link from a question to a workflow plan."@en ;
  rdfs:domain :AuditQuestion ;
  rdfs:range pplan:Plan .

###  https://w3id.org/ai-audit/question#hasQuestion
<https://w3id.org/ai-audit/question#hasQuestion> a owl:ObjectProperty ;
  rdfs:label "has Question"@en ;
  rdfs:comment "Link from System to Question ."@en ;
  rdfs:domain audit:AuditableAISystem ;
  rdfs:range :AuditQuestion .


###  https://w3id.org/ai-audit/question#TraceTemplate
<https://w3id.org/ai-audit/question#TraceTemplate> a owl:Class ;
  rdfs:label "Trace Template"@en ;
  rdfs:comment "Template describing which evidence fields and relations are captured for a given activity/step type."@en .

###  https://w3id.org/ai-audit/question#requiresTraceTemplate
<https://w3id.org/ai-audit/question#requiresTraceTemplate> a owl:ObjectProperty ;
  rdfs:label "requires trace template"@en ;
  rdfs:comment "Binds an audit question to the trace template required to answer it."@en ;
  rdfs:domain :AuditQuestion ;
  rdfs:range :TraceTemplate .

###  https://w3id.org/ai-audit/question#queryLocalPath
  <https://w3id.org/ai-audit/question#queryLocalPath> a owl:DatatypeProperty ;
  rdfs:domain :AuditQuestion ;
  rdfs:range xsd:anyURI .

###  https://w3id.org/ai-audit/question#path
  <https://w3id.org/ai-audit/question#path> a owl:DatatypeProperty ;
  rdfs:domain :TraceTemplate ;
  rdfs:range xsd:anyURI .

### Question Types #############################################################

###  https://w3id.org/ai-audit/question#Lineage_Input
<https://w3id.org/ai-audit/question#Lineage_Input> a :AuditQuestionType ;
  rdfs:label "Input Lineage" .

###  https://w3id.org/ai-audit/question#Accountability
<https://w3id.org/ai-audit/question#Accountability> a :AuditQuestionType ;
  rdfs:label "Accountability" .

###  https://w3id.org/ai-audit/question#Lineage_Output
<https://w3id.org/ai-audit/question#Lineage_Output> a :AuditQuestionType ;
  rdfs:label "Output Lineage" .  

###  https://w3id.org/ai-audit/question#TraceTemplate
<https://w3id.org/ai-audit/question#Temporal> a :AuditQuestionType ;
  rdfs:label "Temporal" .  

###  https://w3id.org/ai-audit/question#Location
<https://w3id.org/ai-audit/question#Location> a :AuditQuestionType ;
    rdfs:label "Location" .

###  https://w3id.org/ai-audit/question#Attribute_Activity
<https://w3id.org/ai-audit/question#Attribute_Activity> a :AuditQuestionType ;
      rdfs:label "Attribute Activity" .

###  https://w3id.org/ai-audit/question#Attribute_Entity
<https://w3id.org/ai-audit/question#Attribute_Entity> a :AuditQuestionType ;
  rdfs:label "Attribute Entity" .

###  https://w3id.org/ai-audit/question#Aggregation
<https://w3id.org/ai-audit/question#Aggregation> a :AuditQuestionType ;
  rdfs:label "Aggregation Entity" .  


